CpcMini/Logos.lean
@@ -473,7 +473,7 @@ def __eo_invoke_cmd_step_pop (s : CState) : CState -> CRule -> CArgList -> CInde
 
 def __eo_invoke_cmd : CState -> CCmd -> CState
   | CState.Stuck, c => CState.Stuck
-  | S, (CCmd.assume_push proven) => (__eo_push_assume_check (__eo_and (__eo_is_bool_type proven) (__eo_is_closed proven)) proven S)
+  | S, (CCmd.assume_push proven) => (__eo_push_assume_check (__eo_is_bool_type proven) proven S)
   | S, (CCmd.check_proven proven) => (__eo_invoke_cmd_check_proven S proven)
   | S, (CCmd.step r args premises) => (__eo_push_proven (__eo_cmd_step_proven S r args premises) S)
   | S, (CCmd.step_pop r args premises) => (__eo_invoke_cmd_step_pop S S r args premises)
